rocq/theories/TypeSystem/EnvRuntimeShadowEvalFacts.v
@@ -382,17 +382,17 @@ Proof.
     assert (Hfresh_s : ~ In x_hidden (store_names s)).
     { apply store_lookup_none_not_in_store_names.
       eapply store_roots_within_lookup_none; eassumption. }
-    dependent destruction H18.
+    dependent destruction H17.
     pose proof (lookup_fn_in_unique_by_name env (fn_name fdef) fdef
-                  H18 eq_refl Hunique) as Hlookup_direct.
+                  H17 eq_refl Hunique) as Hlookup_direct.
     pose proof (lookup_fn_in_unique_by_name env (fn_name fdef) fcallee
                   H5 H6 Hunique) as Hlookup_callee.
     rewrite Hlookup_direct in Hlookup_callee.
     inversion Hlookup_callee; subst fdef.
-	pose proof (typed_args_roots_shadow_safe_roots env Ω n R Σ args
-	                  (apply_lt_params σ (fn_params fcallee))
-	                  Σ' R' arg_roots H21)
-	    as Htyped_args_roots.
+		pose proof (typed_args_roots_shadow_safe_roots env Ω n R Σ args
+		                  (apply_lt_params σ (fn_params fcallee))
+		                  Σ' R' arg_roots H20)
+		    as Htyped_args_roots.
     destruct
       (eval_let_make_closure_captured_call_expr_preserves_typing_with_callee_components_with_preservation_core
         eval_preserves_typing_ready_mutual
@@ -405,15 +405,15 @@ Proof.
         eval_preserves_param_scope_roots_ready_mutual
 	        env Ω n R Σ m x_hidden T_hidden args (fn_name fcallee) captures fcallee σ s s' ret
 	        R' Σ' arg_roots env_lt captured_tys T_body Γ_out R_body
-        roots_body Hstore Hroots Hshadow Hrn Hnamed Hkeys H Heval H9
-        Hnodup_caps H4 Htyped_args_roots H10 H11 H12 H13 H14 H15)
-      as [Hstore' [Hv _]]; eauto.
+        roots_body Hstore Hroots Hshadow Hrn Hnamed Hkeys H Heval H8
+        Hnodup_caps H4 Htyped_args_roots H9 H10 H11 H12 H13 H14
+        Hlookup_direct Hfresh_s H1 H2 H3)
+      as [Hstore' [Hv _]].
     split.
     + exact Hstore'.
-	    + rewrite x in Hv.
-	      eapply VHT_Compatible.
+	    + eapply VHT_Compatible.
       * exact Hv.
-      * apply ty_compatible_b_sound. exact H23.
+      * apply ty_compatible_b_sound. exact H22.
   - dependent destruction Heval.
     + destruct (proj1 eval_preserves_typing_roots_ready_mutual
           env s e1 s1 (VBool true) Heval1 Ω n R Σ T_cond Σ1 R1
@@ -566,17 +566,17 @@ Proof.
     assert (Hfresh_s : ~ In x_hidden (store_names s)).
     { apply store_lookup_none_not_in_store_names.
       eapply store_roots_within_lookup_none; eassumption. }
-    dependent destruction H18.
+    dependent destruction H17.
     pose proof (lookup_fn_in_unique_by_name env (fn_name fdef) fdef
-                  H18 eq_refl Hunique) as Hlookup_direct.
+                  H17 eq_refl Hunique) as Hlookup_direct.
     pose proof (lookup_fn_in_unique_by_name env (fn_name fdef) fcallee
                   H5 H6 Hunique) as Hlookup_callee.
     rewrite Hlookup_direct in Hlookup_callee.
     inversion Hlookup_callee; subst fdef.
-	pose proof (typed_args_roots_shadow_safe_roots env Ω n R Σ args
-	                  (apply_lt_params σ (fn_params fcallee))
-	                  Σ' R' arg_roots H21)
-	    as Htyped_args_roots.
+		pose proof (typed_args_roots_shadow_safe_roots env Ω n R Σ args
+		                  (apply_lt_params σ (fn_params fcallee))
+		                  Σ' R' arg_roots H20)
+		    as Htyped_args_roots.
     destruct
       (eval_let_make_closure_captured_call_expr_preserves_typing_with_callee_components_with_preservation_core
         eval_preserves_typing_ready_mutual
@@ -588,20 +588,20 @@ Proof.
           eval_preserves_typing_roots_ready_prefix_mutual)
         eval_preserves_param_scope_roots_ready_mutual
 	        env Ω n R Σ m x_hidden T_hidden args (fn_name fcallee) captures fcallee σ s s' ret
-        R' Σ' arg_roots env_lt captured_tys T_body Γ_out R_body
-        roots_body Hstore Hroots Hshadow Hrn Hnamed Hkeys H Heval H9
-        Hnodup_caps H4 Htyped_args_roots H10 H11 H12 H13 H14 H15)
-      as [Hstore' [Hv [captured_final [Hcopy Hrooted]]]]; eauto.
+	        R' Σ' arg_roots env_lt captured_tys T_body Γ_out R_body
+        roots_body Hstore Hroots Hshadow Hrn Hnamed Hkeys H Heval H8
+        Hnodup_caps H4 Htyped_args_roots H9 H10 H11 H12 H13 H14
+        Hlookup_direct Hfresh_s H1 H2 H3)
+      as [Hstore' [Hv [captured_final [Hcopy Hrooted]]]].
     pose proof (capture_store_root_sets_bound_from_capture_root_bound
       R s captures (fn_captures fcallee) captured_final capture_roots
-      Hcopy Hroots H16) as Hcap_subset.
+      Hcopy Hroots H15) as Hcap_subset.
     destruct Hrooted as [Hroots' Hvalue_roots Hshadow' Hrn'].
     repeat split.
     + exact Hstore'.
-	    + rewrite x in Hv.
-	      eapply VHT_Compatible.
+	    + eapply VHT_Compatible.
       * exact Hv.
-      * apply ty_compatible_b_sound. exact H23.
+      * apply ty_compatible_b_sound. exact H22.
     + exact Hroots'.
     + eapply value_roots_within_store_subset.
       * exact Hvalue_roots.
